stated principle for proving properties about possible trajectories
generalized from the earlier case when there were no errors.
Also, summarized the error analysis using vectors and pointwise norm and \le

src/robots/car/ackermannSteeringProp.v
@@ -436,31 +436,6 @@ Context {maxTurnCurvature : Qpos}
   End CornersCircle.
     Require Import MCMisc.rings.
 
-  Definition turnRigidStateAtθ (init : Rigid2DState IR) 
-  (tr θ : IR)
-  := 
-  let θi := θ2D init in
-  {|pos2D := pos2D init + {|X:=Sin θ - Sin θi; Y:=Cos θi - Cos θ|}*'tr;
-    θ2D := θ|}.
-
-  Definition turnRigidStateAtDist (init : Rigid2DState IR)
-  (tc: sigT (fun a => apartT a (0:IR))) (d : IR)
-  := 
-  let tr :IR := recipT (projT1 tc) (projT2 tc) in
-  let θi := θ2D init in
-  let θ :IR := θi + (projT1 tc)*d in
-  turnRigidStateAtθ init tr θ.
-
-
-  Global Instance ProperturnRigidStateAtθ: Proper 
-  (equiv ==> equiv ==> equiv ==> equiv) turnRigidStateAtθ.
-  Proof using.
-    intros ? ? H1 ? ? H2 ? ? H3.
-    unfold turnRigidStateAtθ.
-    rewrite H1.
-    rewrite H2.
-    rewrite H3. reflexivity.
-  Qed.
   
   Lemma turnRigidStateAtθCorrect: forall (t :Time)  (p: tstart ≤ t ≤ tend),
     rigidStateAtTime acs t
